Attempt to prove (Invertable <-> Injective /\ Surjective).

ListBackedSet.v
@@ -15,6 +15,36 @@ Definition DecEqPair {S T} : DecEq S -> DecEq T -> DecEq (S * T).
         (right; intro H; inversion H; easy).
     Defined.
 
+Definition Injective {A B} (f : A -> B) := forall x x', f x = f x' -> x = x'.
+Definition Surjective {A B} (f : A -> B) := forall y, exists x, f x = y.
+Definition Invertable {A B} (f : A -> B) := exists g, forall x, g (f x) = x.
+
+Lemma invertable_alternate_characterization {A B}: forall (f : A -> B), Invertable f <-> Injective f /\ Surjective f.
+    unfold Invertable, Injective, Surjective. intro f. split.
+    (* Invertable -> Injective /\ Surjective *)
+    - intros [g g_inv_f]. split.
+        (* Invertable -> Injective *)
+        + intros x x' eq_f. apply (f_equal g) in eq_f. repeat rewrite g_inv_f in eq_f. exact eq_f.
+        (* Invertable -> Surjective *)
+        + intros y. exists (g y).
+            (*Lemma left_implies_right_invertable {A B} (f : A -> B) (g : B -> A) : (forall x, g (f x) = x) -> (forall y, f (g y) = y).
+    (intros g_inv_f y).
+    (set (H := fun x => f_equal f (g_inv_f x))).
+    (set (H' := fun x => f_equal g (f_equal f (g_inv_f x)))).
+    Check g_inv_f (g y).
+    Check (fun x => ltac:(set (tmp := H x); rewrite (g_inv_f) in tmp; exact tmp)).
+    Check (fun x => ltac:(set (tmp := H' x); rewrite (g_inv_f) in tmp; exact tmp)).
+    set (H'' := eq_refl : f (g (f (g y))) = _).
+    rewrite g_inv_f in H'' at 2.
+    set (H''' := eq_refl : g (f (g y)) = _).
+    rewrite g_inv_f in H''' at 2.
+    Show.*)
+    Lemma not_left_implies_right_invertable : ~(forall A B (f : A -> B) (g : B -> A), (forall x, g (f x) = x) -> (forall y, f (g y) = y)).
+        intros H.
+        discriminate (H True bool (fun _ => false) (fun _ => I) (fun x => match x with I => eq_refl end) true).
+        Qed.
+    Abort.
+
 Module ListBackedSet.
     (*Parameter A : Type.
     Parameter eq_dec : forall x y : A, {x = y} + {x <> y}.*)
@@ -119,7 +149,7 @@ Module ListBackedSet'.
             - rewrite ListBackedSet.map_cons. apply Elem_head.
             - apply Elem_tail. exact (IHxs H0).
         Qed.
-    Lemma map_elem' {A B} (f : A -> B) (g : { h : B -> A | forall a, h (f a) = a}) : forall x xs, Elem (f x) (ListBackedSet.map f xs) -> Elem x xs.
+    Lemma map_elem' {A B} (f : A -> B) (g : Invertable f) : forall x xs, Elem (f x) (ListBackedSet.map f xs) -> Elem x xs.
         (* TODO: does this work with something weaker than invertable functions (e.g. surjective)? *)
         intros x xs e.
         destruct g as [g Hg].
